The pass fixed the alignment checking issue: When mem2reg finds eliminatable loads and stores, it does not need to check if their alignments matches the one used by the promotable alloca. If some of them do not use proper-alignments, the original program is undefined. if they match, the values loaded are the same no matter what alignment they use. So, checking alignment is not necessary.
NOTE that the current memory model in high-level assumes all
programs' alignments are correct. 



git-svn-id: https://webdav.seas.upenn.edu/svn/sol/vol@3923 eef5ea85-cc2e-0410-bd84-0fae1f012da8

src3.0/Transforms/alive_store.v
@@ -14,24 +14,33 @@ Require Import trans_tactic.
 
 Import Promotability.
 
-Definition alive_store (sid: id) (v:value) (cs2:cmds) (b:block) (pinfo:PhiInfo)
-  : Prop :=
+(* 
+  An alive store can use a different alignment from the promotable alloca's.
+  If the store's alignment is not legal w.r.t the promotable's, the original
+  program is undefined. Otherwise, the value we load should be the same.
+
+  So far, the memory model assumes all programs' alignments are correct. So,
+  we will not check if an alignment is proper. This is one of our future work.
+*)
+Definition alive_store (sid: id) (sal: align) (v:value) (cs2:cmds) (b:block) 
+  (pinfo:PhiInfo) : Prop :=
 blockInFdefB b (PI_f pinfo) = true /\
 store_in_cmds (PI_id pinfo) cs2 = false /\
 let '(block_intro _ _ cs _) := b in
 exists cs1, exists cs3,
   cs =
   cs1 ++
-  insn_store sid (PI_typ pinfo) v (value_id (PI_id pinfo)) (PI_align pinfo) ::
+  insn_store sid (PI_typ pinfo) v (value_id (PI_id pinfo)) sal ::
   cs2 ++
   cs3.
 
 Record StoreInfo (pinfo: PhiInfo) := mkStoreInfo {
   SI_id : id;
+  SI_align : align;
   SI_value : value;
   SI_tail : cmds;
   SI_block : block;
-  SI_alive : alive_store SI_id SI_value SI_tail SI_block pinfo
+  SI_alive : alive_store SI_id SI_align SI_value SI_tail SI_block pinfo
 }.
 
 Lemma storeinfo_doesnt_use_promotable_allocas: forall pinfo stinfo
@@ -65,7 +74,7 @@ forall cs1 cs3,
   cs0 =
     cs1 ++
     insn_store (SI_id pinfo stinfo) (PI_typ pinfo) (SI_value pinfo stinfo)
-      (value_id (PI_id pinfo)) (PI_align pinfo) ::
+      (value_id (PI_id pinfo)) (SI_align pinfo stinfo) ::
     SI_tail pinfo stinfo ++
     cs3 ->
   (exists csa, exists csb,
@@ -231,7 +240,7 @@ end.
 Ltac destruct_stinfo :=
 match goal with
 | stinfo: StoreInfo _ |- _ =>
-  destruct stinfo as [SI_id0 SI_value0 SI_tail0
+  destruct stinfo as [SI_id0 SI_align0 SI_value0 SI_tail0
                        [SI_l0 SI_ps0 SI_cs0 SI_tmn0] SI_prop0];
   simpl in *;
   destruct SI_prop0 as 
@@ -269,12 +278,12 @@ Local Opaque isReachableFromEntry.
   find_wf_operand_list.
   eapply any_cmd_doesnt_use_following_operands 
     with (c1:=insn_store SI_id0 (PI_typ pinfo) SI_value0
-                 (value_id (PI_id pinfo)) (PI_align pinfo))
+                 (value_id (PI_id pinfo)) SI_align0)
     (l3:=SI_l0)(ps1:=SI_ps0)
     (c:=c)
     (cs:=SI_cs1 ++
              insn_store SI_id0 (PI_typ pinfo) SI_value0
-               (value_id (PI_id pinfo)) (PI_align pinfo) :: 
+               (value_id (PI_id pinfo)) (SI_align0) :: 
              csa ++ c :: cs)(tmn1:=SI_tmn0) in H8; eauto 1.
     clear - H8 H1.
     rewrite getCmdID__getCmdLoc with (id0:=id0) in H8; auto.
