src3.0/Transforms/laa_top.v
@@ -18,34 +18,6 @@ Require Import top_sim.
 Require Import laa.
 Require Import laa_wfS.
 
-Lemma find_st_ld__laainfo: forall l0 ps0 cs0 tmn0 v cs (pinfo:PhiInfo) dones
-  (Hst : ret inr (v, cs) = find_init_stld cs0 (PI_id pinfo) dones)
-  (i1 : id) (Hld : ret inl i1 = find_next_stld cs (PI_id pinfo))
-  (HBinF : blockInFdefB (block_intro l0 ps0 cs0 tmn0) (PI_f pinfo) = true),
-  v = [! pinfo !] /\
-  exists laainfo:LAAInfo pinfo,
-    LAA_lid pinfo laainfo = i1 /\
-    LAA_block pinfo laainfo = (block_intro l0 ps0 cs0 tmn0).
-Proof.
-  intros.
-  assert (v = [! pinfo !] /\
-          exists tail, laa i1 tail (block_intro l0 ps0 cs0 tmn0) pinfo) as Hlaa. 
-    unfold laa.
-    apply find_init_stld_inr_spec in Hst.
-    destruct Hst as [EQ [cs1 Hst]]; subst.
-    apply find_next_stld_inl_spec in Hld.
-    destruct Hld as [cs2 [cs3 [Hld J]]]; subst.
-    split; auto.
-      exists cs2.
-      split; auto.
-      split; auto.
-      exists cs1. exists cs3. auto.
-  destruct Hlaa as [EQ [tail Hlaa]]; subst.
-  split; auto.
-    exists (mkLAAInfo pinfo i1 tail (block_intro l0 ps0 cs0 tmn0) Hlaa).
-    auto.
-Qed.
-
 (* same to las *)
 Lemma s_genInitState__laa_State_simulation: forall pinfo laainfo S1 S2 main
   VarArgs cfg2 IS2
@@ -731,6 +703,46 @@ Proof.
     apply LAA_value__dominates__LAA_lid.
 Qed.
 
+Lemma find_st_ld__laainfo: forall l0 ps0 cs0 tmn0 v cs (pinfo:PhiInfo) dones
+  (Hst : ret inr (v, cs) = find_init_stld cs0 (PI_id pinfo) dones)
+  (i1 : id) (Hld : ret inl i1 = find_next_stld cs (PI_id pinfo))
+  (Hwfpi: WF_PhiInfo pinfo)
+  s m (HwfF: wf_fdef s m (PI_f pinfo)) (Huniq: uniqFdef (PI_f pinfo))
+  (HBinF : blockInFdefB (block_intro l0 ps0 cs0 tmn0) (PI_f pinfo) = true),
+  v = [! pinfo !] /\
+  exists laainfo:LAAInfo pinfo,
+    LAA_lid pinfo laainfo = i1 /\
+    LAA_block pinfo laainfo = (block_intro l0 ps0 cs0 tmn0).
+Proof.
+  intros.
+  assert (v = [! pinfo !] /\
+          exists tail, exists lal, 
+            laa i1 lal tail (block_intro l0 ps0 cs0 tmn0) pinfo) as Hlaa. 
+    unfold laa.
+    apply find_init_stld_inr_spec in Hst.
+    destruct Hst as [cs1 [ty [num [al [EQ Hst]]]]]; subst.
+    apply find_next_stld_inl_spec in Hld.
+    destruct Hld as [cs2 [cs3 [ty' [al' [Hld J]]]]]; subst.
+    assert (J':=HBinF).
+    eapply WF_PhiInfo_spec1' in J'; eauto. inv J'.
+    assert (J':=HBinF).
+    match goal with
+    | H1 : context [?A ++ ?b :: ?C ++ ?d :: ?E] |- _ =>
+      rewrite_env ((A ++ b :: C) ++ d :: E) in H1;
+      eapply WF_PhiInfo_spec23 in H1; eauto
+    end.
+    subst. 
+    split; auto.
+      exists cs2. exists al'.
+      split; auto.
+      split; auto.
+      exists cs1. exists cs3. auto.
+  destruct Hlaa as [EQ [tail [lal Hlaa]]]; subst.
+  split; auto.
+    exists (mkLAAInfo pinfo i1 lal tail (block_intro l0 ps0 cs0 tmn0) Hlaa).
+    auto.
+Qed.
+
 Lemma laa_sim: forall (los : layouts) (nts : namedts) (fh : fheader)
   (dones : list id) (pinfo : PhiInfo) (main : id) (VarArgs : list (GVsT DGVs))
   (bs1 : list block) (l0 : l) (ps0 : phinodes) (cs0 : cmds) (tmn0 : terminator)
@@ -760,6 +772,12 @@ Proof.
   assert (blockInFdefB (block_intro l0 ps0 cs0 tmn0) (PI_f pinfo) = true)
     as HBinF.
     rewrite Heq. simpl. apply InBlocksB_middle.
+  assert (wf_fdef [module_intro los nts (Ps1++product_fdef (PI_f pinfo)::Ps2)]
+            (module_intro los nts (Ps1++product_fdef (PI_f pinfo)::Ps2)) 
+            (PI_f pinfo) /\ uniqFdef (PI_f pinfo)) as J.
+    rewrite Heq in *. subst.
+    apply wf_single_system__wf_uniq_fdef; auto.
+  destruct J as [HwfF HuniqF].
   eapply find_st_ld__laainfo in HBinF; eauto.
   destruct HBinF as [EQ [laainfo [J1 J2]]]; subst.
   assert (Huniq:=HwfS). apply wf_system__uniqSystem in Huniq; auto.
@@ -779,9 +797,6 @@ Proof.
     simpl in Huniq. destruct Huniq as [[_ [_ Huniq]] _].
     unfold TopSim.products_simulation. unfold fsim. unfold Fsim. 
     apply uniq_products_simulation; auto.
-  assert (uniqFdef (PI_f pinfo)) as HuniqF.
-    rewrite Heq in *.
-    eapply wf_single_system__wf_uniq_fdef; eauto.
 
 Ltac laa_sim_init :=
 match goal with
