src3.0/Transforms/las_top.v
@@ -454,33 +454,6 @@ Proof.
       erewrite TopSim.lookupExFdecViaPtr__simulation_None_r2l; eauto.
 Qed.
 
-Lemma find_st_ld__lasinfo: forall l0 ps0 cs0 tmn0 i0 v cs (pinfo:PhiInfo) dones
-  (Hst : ret inl (i0, v, cs) = find_init_stld cs0 (PI_id pinfo) dones)
-  (i1 : id) (Hld : ret inl i1 = find_next_stld cs (PI_id pinfo))
-  (HBinF : blockInFdefB (block_intro l0 ps0 cs0 tmn0) (PI_f pinfo) = true),
-  exists lasinfo:LASInfo pinfo,
-    LAS_lid pinfo lasinfo = i1 /\
-    LAS_sid pinfo lasinfo = i0 /\
-    LAS_value pinfo lasinfo = v /\
-    LAS_block pinfo lasinfo = (block_intro l0 ps0 cs0 tmn0).
-Proof.
-  intros.
-  assert (exists tail, las i1 i0 v tail (block_intro l0 ps0 cs0 tmn0) pinfo)
-    as Hlas. 
-    unfold las.
-    apply find_init_stld_inl_spec in Hst.
-    destruct Hst as [cs1 Hst]; subst.
-    apply find_next_stld_inl_spec in Hld.
-    destruct Hld as [cs2 [cs3 [Hld J]]]; subst.
-    exists cs2.
-    split; auto.
-    split; auto.
-    exists cs1. exists cs3. auto.
-  destruct Hlas as [tail Hlas].
-  exists (mkLASInfo pinfo i1 i0 v tail (block_intro l0 ps0 cs0 tmn0) Hlas).
-  auto.
-Qed.
-
 Lemma las_is_bsim : forall pinfo lasinfo Cfg1 St1 Cfg2 St2 St2' tr2 
   (Hwfpi: WF_PhiInfo pinfo) 
   (Hwfcfg: OpsemPP.wf_Config Cfg1) (Hwfpp: OpsemPP.wf_State Cfg1 St1) 
@@ -701,6 +674,45 @@ Proof.
     alive_store.preservation_plus.
 Qed.
 
+Lemma find_st_ld__lasinfo: forall l0 ps0 cs0 tmn0 i0 v cs (pinfo:PhiInfo) dones
+  (Hst : ret inl (i0, v, cs) = find_init_stld cs0 (PI_id pinfo) dones)
+  (i1 : id) (Hld : ret inl i1 = find_next_stld cs (PI_id pinfo)) 
+  (Hwfpi: WF_PhiInfo pinfo)
+  s m (HwfF: wf_fdef s m (PI_f pinfo)) (Huniq: uniqFdef (PI_f pinfo))
+  (HBinF : blockInFdefB (block_intro l0 ps0 cs0 tmn0) (PI_f pinfo) = true),
+  exists lasinfo:LASInfo pinfo,
+    LAS_lid pinfo lasinfo = i1 /\
+    LAS_sid pinfo lasinfo = i0 /\
+    LAS_value pinfo lasinfo = v /\
+    LAS_block pinfo lasinfo = (block_intro l0 ps0 cs0 tmn0).
+Proof.
+  intros.
+  assert (exists tail, exists lalign, exists salign, 
+            las i1 i0 lalign salign v tail (block_intro l0 ps0 cs0 tmn0) pinfo)
+    as Hlas. 
+    unfold las.
+    apply find_init_stld_inl_spec in Hst.
+    destruct Hst as [cs1 [ty1 [al1 Hst]]]; subst.
+    apply find_next_stld_inl_spec in Hld.
+    destruct Hld as [cs2 [cs3 [tl2 [al2 [Hld J]]]]]; subst.
+    exists cs2. exists al2. exists al1.
+    split; auto.
+    split; auto.
+    exists cs1. exists cs3.
+      assert (J':=HBinF).
+      eapply WF_PhiInfo_spec24 in J'; eauto.
+      match goal with
+      | H1 : context [?A ++ ?b :: ?C ++ ?d :: ?E] |- _ =>
+        rewrite_env ((A ++ b :: C) ++ d :: E) in H1;
+        eapply WF_PhiInfo_spec23 in H1; eauto
+      end.
+      subst. auto.
+  destruct Hlas as [tail [lal [sal Hlas]]].
+  exists 
+    (mkLASInfo pinfo i1 i0 lal sal v tail (block_intro l0 ps0 cs0 tmn0) Hlas).
+  auto.
+Qed.
+
 Lemma las_sim: forall (los : layouts) (nts : namedts) (fh : fheader)
   (dones : list id) (pinfo: PhiInfo) (main : id) (VarArgs : list (GVsT DGVs))
   (bs1 : list block) (l0 : l) (ps0 : phinodes) (cs0 : cmds) (tmn0 : terminator)
@@ -728,8 +740,15 @@ Proof.
   assert (blockInFdefB (block_intro l0 ps0 cs0 tmn0) (PI_f pinfo) = true)
     as HBinF.
     rewrite Heq. simpl. apply InBlocksB_middle.
+  assert (wf_fdef [module_intro los nts (Ps1++product_fdef (PI_f pinfo)::Ps2)]
+            (module_intro los nts (Ps1++product_fdef (PI_f pinfo)::Ps2)) 
+            (PI_f pinfo) /\ uniqFdef (PI_f pinfo)) as J.
+    rewrite Heq in *.
+    apply wf_single_system__wf_uniq_fdef; auto.
+  destruct J as [HwfF HuniqF].
   eapply find_st_ld__lasinfo in HBinF; eauto.
   destruct HBinF as [lasinfo [J1 [J2 [J3 J4]]]]; subst.
+
   assert (Huniq:=HwfS). apply wf_system__uniqSystem in Huniq; auto.
   assert (system_simulation pinfo lasinfo
      [module_intro los nts
@@ -747,13 +766,6 @@ Proof.
     simpl in Huniq. destruct Huniq as [[_ [_ Huniq]] _].
     unfold TopSim.products_simulation. unfold fsim. unfold Fsim.
     apply uniq_products_simulation; auto.
-
-  assert (wf_fdef [module_intro los nts (Ps1++product_fdef (PI_f pinfo)::Ps2)]
-            (module_intro los nts (Ps1++product_fdef (PI_f pinfo)::Ps2)) 
-            (PI_f pinfo) /\ uniqFdef (PI_f pinfo)) as J.
-    rewrite Heq in *.
-    apply wf_single_system__wf_uniq_fdef; auto.
-  destruct J as [HwfF HuniqF].
 
 Ltac las_sim_init :=
 match goal with
